Adding lemmas

poSTVM/poSTVM_alt_inductive.thy
@@ -25,7 +25,7 @@ datatype stmt =
   FBInvocation fb_invocation |
   Return |
   Exit |
-  ProcessSt process_contextment |
+  ProcessSt process_statement |
   SetStateSt set_state_statement |
   ResetSt |
   IfSt expr stmt stmt |
@@ -35,174 +35,228 @@ datatype stmt =
 *)
 
 text "exec process statement"
-definition update_process_status :: "model_context \<Rightarrow> process_contextment \<Rightarrow>(statement_result* model_context)" where
+definition update_process_status :: "model_context \<Rightarrow> process_statement \<Rightarrow>(statement_result* model_context)" where
 "update_process_status st ps =
   (case ps of
-    process_contextment.Start name_option \<Rightarrow> 
+    process_statement.Start name_option \<Rightarrow> 
       (case name_option of
         None \<Rightarrow> (statement_result.Return, reset_cur_process st)
       | Some name \<Rightarrow> (statement_result.Continue, reset_process st name))
-  | process_contextment.Stop name_option \<Rightarrow> 
+  | process_statement.Stop name_option \<Rightarrow> 
       (case name_option of
         None \<Rightarrow> (statement_result.Return, stop_cur_process st)
       | Some name \<Rightarrow> (statement_result.Continue, stop_process st name))
-  | process_contextment.Error name_option \<Rightarrow> 
+  | process_statement.Error name_option \<Rightarrow> 
       (case name_option of
         None \<Rightarrow> (statement_result.Return, error_cur_process st)
   | Some name \<Rightarrow> (statement_result.Continue, error_process st name)))"
 declare update_process_status_def [simp]
 
 inductive 
-  eval :: "[model_context, expr, basic_post_type] \<Rightarrow> bool" ("_ \<turnstile> _ \<rightarrow> _") and
-  exec :: "[statement_result * model_context,stmt,statement_result * model_context] \<Rightarrow> bool" ("_ \<turnstile> _ \<longrightarrow> _") and
+  eval :: "[model_context, expr, model_context * basic_post_type] \<Rightarrow> bool" ("_ \<turnstile> _ \<rightarrow> _") and
+  exec :: "[model_context,stmt,model_context] \<Rightarrow> bool" ("_ \<turnstile> _ \<longrightarrow> _") and
   exec_func :: "[model_context,func_name,func_params,model_context*basic_post_type] \<Rightarrow> bool" ("_\<turnstile>_,_\<longrightarrow> _") and
   assign_param :: "[model_context,assign_type,param_assign list,model_context,model_context] \<Rightarrow> bool"
   where
-    BinOp : "\<lbrakk>st\<turnstile>exp1\<rightarrow>val1;
-              st\<turnstile>exp2\<rightarrow>val2;
+    BinOp : "\<lbrakk>st\<turnstile>exp1\<rightarrow>(st1,val1);
+              st1\<turnstile>exp2\<rightarrow>(st2,val2);
               val = binary_op_exec bin_op val1 val2 \<rbrakk> \<Longrightarrow>
-             st\<turnstile>expr.Binary bin_op exp1 exp2\<rightarrow>val"
-  | UnOp : "\<lbrakk>st\<turnstile>pexp\<rightarrow>val1;
+             st\<turnstile>expr.Binary bin_op exp1 exp2\<rightarrow>(st2,val)"
+  | UnOp : "\<lbrakk>st\<turnstile>pexp\<rightarrow>(st1,val1);
                 val = (unary_op_exec un_op val1)\<rbrakk> \<Longrightarrow>
-               st\<turnstile> expr.Unary un_op pexp\<rightarrow>val"
+               st\<turnstile> expr.Unary un_op pexp\<rightarrow>(st1,val)"
   | Const : "\<lbrakk>val = const_to_basic c\<rbrakk>\<Longrightarrow>
-            st\<turnstile>expr.Const c\<rightarrow>val"
+            st\<turnstile>expr.Const c\<rightarrow>(st,val)"
   | Var :  "\<lbrakk>val = get_cur_symbvar_by_name st var_name\<rbrakk>\<Longrightarrow>
-           st\<turnstile>expr.SymbolicVar var_name\<rightarrow>val"
-  | ArrayVar : "\<lbrakk>st\<turnstile>exp\<rightarrow>pos;
+           st\<turnstile>expr.SymbolicVar var_name\<rightarrow>(st,val)"
+  | ArrayVar : "\<lbrakk>st\<turnstile>exp\<rightarrow>(_,pos);
                  val = get_cur_arvar_by_name_by_pos st var_name pos\<rbrakk>\<Longrightarrow>
-               st\<turnstile>expr.ArrayVar var_name exp\<rightarrow>val"
+               st\<turnstile>expr.ArrayVar var_name exp\<rightarrow>(st,val)"
   | PSE : "\<lbrakk>val = check_proc_status st p_name p_status\<rbrakk>\<Longrightarrow>
-          st\<turnstile>expr.ProcStatEpxr p_name p_status\<rightarrow>val"
+          st\<turnstile>expr.ProcStatEpxr p_name p_status\<rightarrow>(st,val)"
+ |FuncCall : "\<lbrakk>st\<turnstile>name,as_list\<longrightarrow>(st1,val)\<rbrakk> \<Longrightarrow> st\<turnstile>expr.FunctionCall name as_list \<rightarrow> (st1,val)"
 
-  | Blank : "(res,st)\<turnstile>stmt.Blank\<longrightarrow>(res,st)"
-  | Comb : "\<lbrakk>st\<turnstile>s1\<longrightarrow>st_res1;
-             (st_res1)\<turnstile>(case (fst st_res1) of
-                          (statement_result.Continue) \<Rightarrow> s2
-                        | (res) \<Rightarrow> stmt.Blank)\<longrightarrow>st2 \<rbrakk>\<Longrightarrow>
-           st\<turnstile>stmt.Comb s1 s2 \<longrightarrow> st2"
-  | If : "\<lbrakk>(snd st)\<turnstile>exp\<rightarrow>val;
-            st\<turnstile>(if (basic_post_type_to_bool val) then s1 else s2)\<longrightarrow>st1\<rbrakk>\<Longrightarrow>
+  | Blank : "st\<turnstile>stmt.Blank\<longrightarrow>st"
+  | Comb : "\<lbrakk>st\<turnstile>s1\<longrightarrow>st1;
+             st1\<turnstile>s2\<longrightarrow>st2\<rbrakk>\<Longrightarrow>
+           st\<turnstile>stmt.Comb s1 s2 \<longrightarrow>st2"
+  | IfT : "\<lbrakk>st\<turnstile>exp\<rightarrow>(st_res,val);
+            (basic_post_type_to_bool val);
+            st\<turnstile>s1\<longrightarrow>st1\<rbrakk>\<Longrightarrow>
          st\<turnstile>stmt.IfSt exp s1 s2\<longrightarrow>st1"
-  | LoopF : "\<lbrakk>(snd st)\<turnstile>exp\<rightarrow>val; \<not>(basic_post_type_to_bool val)\<rbrakk>\<Longrightarrow>
+  | IfF : "\<lbrakk>st\<turnstile>exp\<rightarrow>(st_res,val);
+           \<not>(basic_post_type_to_bool val);
+           st\<turnstile>s2\<longrightarrow>st1\<rbrakk> \<Longrightarrow> st\<turnstile>stmt.IfSt exp s1 s2\<longrightarrow>st1"
+  | LoopF : "\<lbrakk>st\<turnstile>exp\<rightarrow>(st_sub,val); \<not>(basic_post_type_to_bool val)\<rbrakk>\<Longrightarrow>
             st\<turnstile>stmt.WhileSt exp s\<longrightarrow>st"
-  | LoopT : "\<lbrakk>(snd st)\<turnstile>exp\<rightarrow>val; (basic_post_type_to_bool val);
+  | LoopT : "\<lbrakk>st\<turnstile>exp\<rightarrow>(st_sub,val); (basic_post_type_to_bool val);
               st\<turnstile>s\<longrightarrow>st1;st1\<turnstile>stmt.WhileSt exp s\<longrightarrow>st2\<rbrakk>\<Longrightarrow>
-            st\<turnstile>stmt.WhileSt exp s\<longrightarrow>st2"
-  | AssignS : "\<lbrakk>(snd st)\<turnstile>exp\<rightarrow>val;
-                st1 = (set_symbvar (snd st) var_name val)\<rbrakk>\<Longrightarrow>
-              st\<turnstile>stmt.AssignSt (common_var.Symbolic var_name) exp\<longrightarrow>(statement_result.Continue, st1)"
-  | AssignA : "\<lbrakk>(snd st)\<turnstile>exp\<rightarrow>val1;
-                (snd st)\<turnstile>pos\<rightarrow>val2;
-                st1 = (set_arvar (snd st) var_name val2 val1)\<rbrakk>\<Longrightarrow>
-              st\<turnstile>stmt.AssignSt (common_var.Array var_name pos) exp\<longrightarrow>(statement_result.Continue, st1)"
-  | Return : "st\<turnstile>stmt.Return\<longrightarrow>(statement_result.Continue, snd st)"
-  | Exit : "st\<turnstile>stmt.Exit\<longrightarrow>(statement_result.Continue, snd st)"
-  | Process : "\<lbrakk>st2 = (update_process_status (snd st) ps)\<rbrakk>\<Longrightarrow>
-                st\<turnstile>stmt.ProcessSt ps\<longrightarrow>st2"
+              st\<turnstile>stmt.WhileSt exp s\<longrightarrow>st2"
+  | AssignS : "\<lbrakk>st\<turnstile>exp\<rightarrow>(st1,val);
+                st2 = (set_symbvar st1 var_name val)\<rbrakk>\<Longrightarrow>
+              st\<turnstile>stmt.AssignSt (common_var.Symbolic var_name) exp\<longrightarrow>st2"
+  | AssignA : "\<lbrakk>st\<turnstile>exp\<rightarrow>(st1,val1);
+                st1\<turnstile>pos\<rightarrow>(st1,val2);
+                st2 = (set_arvar st1 var_name val2 val1)\<rbrakk>\<Longrightarrow>
+              st\<turnstile>stmt.AssignSt (common_var.Array var_name pos) exp\<longrightarrow>st2"
+  | Return : "st\<turnstile>stmt.Return\<longrightarrow>st"
+  | Exit : "st\<turnstile>stmt.Exit\<longrightarrow>st"
+  | ProcessStart : "\<lbrakk>st1 = (case stm_name_option of None \<Rightarrow> reset_cur_process st | Some name \<Rightarrow> reset_process st name)\<rbrakk> \<Longrightarrow> 
+                    st\<turnstile>stmt.ProcessSt (process_statement.Start stm_name_option)\<longrightarrow>st1"
+  | ProcessStop : "\<lbrakk>st1 = (case stm_name_option of None \<Rightarrow> stop_cur_process st | Some name \<Rightarrow> stop_process st name)\<rbrakk> \<Longrightarrow> 
+                    st\<turnstile>stmt.ProcessSt (process_statement.Start stm_name_option)\<longrightarrow>st1"
+  | ProcessError : "\<lbrakk>st1 = (case stm_name_option of None \<Rightarrow> error_cur_process st | Some name \<Rightarrow> error_process st name)\<rbrakk> \<Longrightarrow> 
+                    st\<turnstile>stmt.ProcessSt (process_statement.Start stm_name_option)\<longrightarrow>st1"
   | SetState : "\<lbrakk>st1 = (case st_name_option of
-                        None \<Rightarrow> (statement_result.Continue, set_next_state_next (snd st))
-                      | Some name \<Rightarrow> (statement_result.Continue, set_state (snd st) name))\<rbrakk>\<Longrightarrow>
+                        None \<Rightarrow> (set_next_state_next st)
+                      | Some name \<Rightarrow> (set_state st name))\<rbrakk>\<Longrightarrow>
                 st\<turnstile>stmt.SetStateSt st_name_option\<longrightarrow>st1"
-  | Reset : "\<lbrakk>st1 = reset_cur_timer(snd st)\<rbrakk> \<Longrightarrow> st\<turnstile>stmt.ResetSt\<longrightarrow>(statement_result.Continue,st1)"
+  | Reset : "\<lbrakk>st1 = reset_cur_timer st\<rbrakk> \<Longrightarrow> st\<turnstile>stmt.ResetSt\<longrightarrow>st1"
 
   | FuncStep : "\<lbrakk>(f_name,res,vars,stmts) = (get_func_by_name st name);
                   proxy_state = (gen_proxy_for_func st (f_name,res,vars,stmts));
                   assign_param st assign_type.ColonEq params proxy_state as_proxy_state;
-                  (statement_result.Continue, as_proxy_state)\<turnstile>stmts\<longrightarrow>(st_res,st1);
+                  as_proxy_state\<turnstile>stmts\<longrightarrow>st1;
                   assign_param st1 assign_type.Conseq params st new_st;
                   res = (get_cur_symbvar_by_name st1 f_name)\<rbrakk>\<Longrightarrow>
                 st\<turnstile>name,params\<longrightarrow>(new_st,res)"
   | AssignPNill : "assign_param base_st type [] st st"
-  | AssignPConsCol : "\<lbrakk>base_st \<turnstile> exp \<rightarrow> val;
+  | AssignPConsCol : "\<lbrakk>base_st \<turnstile> exp \<rightarrow> (st,val);
                        (if as_type = assign_type.ColonEq 
                         then (assign_param base_st assign_type.ColonEq other (set_symbvar st name val) new_st)
                         else (assign_param base_st assign_type.ColonEq other st new_st))\<rbrakk> \<Longrightarrow> 
                       assign_param base_st assign_type.ColonEq ((param_assign.SymbolicVar name as_type exp)#other) st new_st"
-  | AssignPConsCon : "\<lbrakk>base_st \<turnstile> exp \<rightarrow> val;
+  | AssignPConsCon : "\<lbrakk>base_st \<turnstile> exp \<rightarrow> (st,val);
                        (if as_type = assign_type.Conseq 
                         then (assign_param base_st assign_type.Conseq other st new_st) 
                         else (assign_param base_st assign_type.Conseq other (set_symbvar st name val) new_st))  \<rbrakk> \<Longrightarrow> 
                       assign_param base_st assign_type.Conseq ((param_assign.SymbolicVar name as_type exp)#other) st new_st"
 
-lemma [code_pred_intro blank]: "(res,st)\<turnstile>stmt.Blank\<longrightarrow>(res,st)"
-  by (simp add:eval_exec_exec_func_assign_param.Blank )
-lemma [code_pred_intro comb]:
-"\<lbrakk>st\<turnstile>s1\<longrightarrow>st_res1;
-             (st_res1)\<turnstile>(case (fst st_res1) of
-                          (statement_result.Continue) \<Rightarrow> s2
-                        | (res) \<Rightarrow> stmt.Blank)\<longrightarrow>st2 \<rbrakk>\<Longrightarrow>
-           st\<turnstile>stmt.Comb s1 s2 \<longrightarrow> st2"
-  by (simp add: eval_exec_exec_func_assign_param.Comb)
-lemma [code_pred_intro ifs]:
-"\<lbrakk>(snd st)\<turnstile>exp\<rightarrow>val;
-            st\<turnstile>(if (basic_post_type_to_bool val) then s1 else s2)\<longrightarrow>st1\<rbrakk>\<Longrightarrow>
-         st\<turnstile>stmt.IfSt exp s1 s2\<longrightarrow>st1"
-  by (simp add: eval_exec_exec_func_assign_param.If)
+print_theorems 
 
-
-lemma [code_pred_intro true_loop]:
-  "\<lbrakk>(snd st)\<turnstile>exp\<rightarrow>val; (basic_post_type_to_bool val);
-              st\<turnstile>s\<longrightarrow>st1;st1\<turnstile>stmt.WhileSt exp s\<longrightarrow>st2\<rbrakk>\<Longrightarrow>
-            st\<turnstile>stmt.WhileSt exp s\<longrightarrow>st2"
-  by (simp add: eval_exec_exec_func_assign_param.LoopT)
-lemma [code_pred_intro false_loop]:
-  "\<lbrakk>(snd st)\<turnstile>exp\<rightarrow>val; \<not>(basic_post_type_to_bool val)\<rbrakk>\<Longrightarrow>
-            st\<turnstile>stmt.WhileSt exp s\<longrightarrow>st"
-  by (simp add: eval_exec_exec_func_assign_param.LoopF)
-
+text "eval code_pred_intro lemmas"
 lemma [code_pred_intro]: 
-"\<lbrakk>(snd st)\<turnstile>exp\<rightarrow>val; (basic_post_type_to_bool val);
-              st\<turnstile>s\<longrightarrow>st1;st1\<turnstile>stmt.WhileSt exp s\<longrightarrow>st2\<rbrakk>\<Longrightarrow>
-            st\<turnstile>stmt.WhileSt exp s\<longrightarrow>st2"
- "\<lbrakk>(snd st)\<turnstile>exp\<rightarrow>val; \<not>(basic_post_type_to_bool val)\<rbrakk>\<Longrightarrow>
-            st\<turnstile>stmt.WhileSt exp s\<longrightarrow>st"
+"\<lbrakk>st\<turnstile>exp1\<rightarrow>(st1,val1);
+              st1\<turnstile>exp2\<rightarrow>(st2,val2);
+              val = binary_op_exec bin_op val1 val2 \<rbrakk> \<Longrightarrow>
+             st\<turnstile>expr.Binary bin_op exp1 exp2\<rightarrow>(st2,val)"
+"\<lbrakk>st\<turnstile>pexp\<rightarrow>(st1,val1);
+                val = (unary_op_exec un_op val1)\<rbrakk> \<Longrightarrow>
+               st\<turnstile> expr.Unary un_op pexp\<rightarrow>(st1,val)"
+"\<lbrakk>val = const_to_basic c\<rbrakk>\<Longrightarrow>
+            st\<turnstile>expr.Const c\<rightarrow>(st,val)"
+"\<lbrakk>val = get_cur_symbvar_by_name st var_name\<rbrakk>\<Longrightarrow>
+           st\<turnstile>expr.SymbolicVar var_name\<rightarrow>(st,val)"
+"\<lbrakk>st\<turnstile>exp\<rightarrow>(st1,pos);
+                 val = get_cur_arvar_by_name_by_pos st var_name pos\<rbrakk>\<Longrightarrow>
+               st\<turnstile>expr.ArrayVar var_name exp\<rightarrow>(st,val)"
+"\<lbrakk>val = check_proc_status st p_name p_status\<rbrakk>\<Longrightarrow>
+          st\<turnstile>expr.ProcStatEpxr p_name p_status\<rightarrow>(st,val)"
+"\<lbrakk>st\<turnstile>name,as_list\<longrightarrow>(st1,val)\<rbrakk> \<Longrightarrow> st\<turnstile>expr.FunctionCall name as_list \<rightarrow> (st1,val)"
   by (auto intro: eval_exec_exec_func_assign_param.intros)
 
-lemma [code_pred_intro assigns]:
-"\<lbrakk>(snd st)\<turnstile>exp\<rightarrow>val;
-                st1 = (set_symbvar (snd st) var_name val)\<rbrakk>\<Longrightarrow>
-              st\<turnstile>stmt.AssignSt (common_var.Symbolic var_name) exp\<longrightarrow>(statement_result.Continue, st1)"
-  by (simp add: eval_exec_exec_func_assign_param.AssignS)
-lemma [code_pred_intro assigna]:
-"\<lbrakk>(snd st)\<turnstile>exp\<rightarrow>val1;
-                (snd st)\<turnstile>pos\<rightarrow>val2;
-                st1 = (set_arvar (snd st) var_name val2 val1)\<rbrakk>\<Longrightarrow>
-              st\<turnstile>stmt.AssignSt (common_var.Array var_name pos) exp\<longrightarrow>(statement_result.Continue, st1)"
-  by (simp add: eval_exec_exec_func_assign_param.AssignA)
-lemma [code_pred_intro return]:
-"st\<turnstile>stmt.Return\<longrightarrow>(statement_result.Continue, snd st)"
-  by (simp add: eval_exec_exec_func_assign_param.Return)
-lemma [code_pred_intro exit]:
-"st\<turnstile>stmt.Exit\<longrightarrow>(statement_result.Continue, snd st)"
-  by (simp add: eval_exec_exec_func_assign_param.Exit)
-lemma [code_pred_intro process]:
-"\<lbrakk>st2 = (update_process_status (snd st) ps)\<rbrakk>\<Longrightarrow>
-                st\<turnstile>stmt.ProcessSt ps\<longrightarrow>st2"
-  by (simp add: eval_exec_exec_func_assign_param.Process)
-lemma [code_pred_intro set_state]:
-"\<lbrakk>st1 = (case st_name_option of
-                        None \<Rightarrow> (statement_result.Continue, set_next_state_next (snd st))
-                      | Some name \<Rightarrow> (statement_result.Continue, set_state (snd st) name))\<rbrakk>\<Longrightarrow>
-                st\<turnstile>stmt.SetStateSt st_name_option\<longrightarrow>st1"
-  by (simp add: eval_exec_exec_func_assign_param.SetState)
-lemma [code_pred_intro reset]:
-"\<lbrakk>st1 = reset_cur_timer(snd st)\<rbrakk> \<Longrightarrow> st\<turnstile>stmt.ResetSt\<longrightarrow>(statement_result.Continue,st1)"
-  by (simp add: eval_exec_exec_func_assign_param.Reset)
+inductive_cases BinOpE[elim!]: "st\<turnstile>expr.Binary bin_op exp1 exp2\<rightarrow>(st2,val)"
+inductive_cases UnOpE[elim!]: "st\<turnstile> expr.Unary un_op pexp\<rightarrow>(st1,val)"
+inductive_cases ConstE[elim!]: "st\<turnstile>expr.Const c\<rightarrow>(st,val)"
+inductive_cases VarE[elim!]: "st\<turnstile>expr.SymbolicVar var_name\<rightarrow>(st,val)"
+inductive_cases ArrayVarE[elim!]: "st\<turnstile>expr.ArrayVar var_name exp\<rightarrow>(st,val)"
+inductive_cases PSE[elim!]: "st\<turnstile>expr.ProcStatEpxr p_name p_status\<rightarrow>(st,val)"
+inductive_cases FuncCallE[elim!]: "st\<turnstile>expr.FunctionCall name as_list \<rightarrow> (st1,val)"
 
+text "exec code_pred_intro lemmas"
+lemma [code_pred_intro]:
+"st\<turnstile>stmt.Blank\<longrightarrow>st"
+"\<lbrakk>st\<turnstile>s1\<longrightarrow>st1;
+             st1\<turnstile>s2\<longrightarrow>st2\<rbrakk>\<Longrightarrow>
+           st\<turnstile>stmt.Comb s1 s2 \<longrightarrow>st2"
+"\<lbrakk>st\<turnstile>exp\<rightarrow>(st_res,val);
+            (basic_post_type_to_bool val);
+            st\<turnstile>s1\<longrightarrow>st1\<rbrakk>\<Longrightarrow>
+         st\<turnstile>stmt.IfSt exp s1 s2\<longrightarrow>st1"
+"\<lbrakk>st\<turnstile>exp\<rightarrow>(st_res,val);
+           \<not>(basic_post_type_to_bool val);
+           st\<turnstile>s2\<longrightarrow>st1\<rbrakk> \<Longrightarrow> st\<turnstile>stmt.IfSt exp s1 s2\<longrightarrow>st1"
+"\<lbrakk>st\<turnstile>exp\<rightarrow>(st1,val); \<not>(basic_post_type_to_bool val)\<rbrakk>\<Longrightarrow>
+            st\<turnstile>stmt.WhileSt exp s\<longrightarrow>st"
+"\<lbrakk>st\<turnstile>exp\<rightarrow>(st1,val); (basic_post_type_to_bool val);
+              st\<turnstile>s\<longrightarrow>st1;st1\<turnstile>stmt.WhileSt exp s\<longrightarrow>st2\<rbrakk>\<Longrightarrow>
+              st\<turnstile>stmt.WhileSt exp s\<longrightarrow>st2"
+"\<lbrakk>st\<turnstile>exp\<rightarrow>(st1,val);
+                st2 = (set_symbvar st1 var_name val)\<rbrakk>\<Longrightarrow>
+              st\<turnstile>stmt.AssignSt (common_var.Symbolic var_name) exp\<longrightarrow>st2"
+"\<lbrakk>st\<turnstile>exp\<rightarrow>(st1,val1);
+                st1\<turnstile>pos\<rightarrow>(st1,val2);
+                st2 = (set_arvar st1 var_name val2 val1)\<rbrakk>\<Longrightarrow>
+              st\<turnstile>stmt.AssignSt (common_var.Array var_name pos) exp\<longrightarrow>st2"
+"st\<turnstile>stmt.Return\<longrightarrow>st"
+"st\<turnstile>stmt.Exit\<longrightarrow>st"
+"\<lbrakk>st1 = (case stm_name_option of None \<Rightarrow> reset_cur_process st | Some name \<Rightarrow> reset_process st name)\<rbrakk> \<Longrightarrow> 
+                    st\<turnstile>stmt.ProcessSt (process_statement.Start stm_name_option)\<longrightarrow>st1"
+"\<lbrakk>st1 = (case stm_name_option of None \<Rightarrow> stop_cur_process st | Some name \<Rightarrow> stop_process st name)\<rbrakk> \<Longrightarrow> 
+                    st\<turnstile>stmt.ProcessSt (process_statement.Start stm_name_option)\<longrightarrow>st1"
+"\<lbrakk>st1 = (case stm_name_option of None \<Rightarrow> error_cur_process st | Some name \<Rightarrow> error_process st name)\<rbrakk> \<Longrightarrow> 
+                    st\<turnstile>stmt.ProcessSt (process_statement.Start stm_name_option)\<longrightarrow>st1"
+"\<lbrakk>st1 = (case st_name_option of
+                        None \<Rightarrow> (set_next_state_next st)
+                      | Some name \<Rightarrow> (set_state st name))\<rbrakk>\<Longrightarrow>
+                st\<turnstile>stmt.SetStateSt st_name_option\<longrightarrow>st1"
+"\<lbrakk>st1 = reset_cur_timer st\<rbrakk> \<Longrightarrow> st\<turnstile>stmt.ResetSt\<longrightarrow>st1"
+  by (auto intro: eval_exec_exec_func_assign_param.intros)
+
+inductive_cases BlankE[elim!]: "st\<turnstile>stmt.Blank\<longrightarrow>st1"
+thm BlankE
+inductive_cases CombE[elim!]: "st\<turnstile>stmt.Comb s1 s2 \<longrightarrow>st2"
+thm CombE
+inductive_cases IfE[elim!]: "st\<turnstile>stmt.IfSt exp s1 s2\<longrightarrow>st1"
+thm IfE
+inductive_cases LoopE[elim!]: "st\<turnstile>stmt.WhileSt exp s\<longrightarrow>st2"
+thm LoopE
+inductive_cases AssignE[elim!]: "st\<turnstile>stmt.AssignSt v exp\<longrightarrow>st2"
+inductive_cases ReturnE[elim!]: "st\<turnstile>stmt.Return\<longrightarrow>st"
+inductive_cases ExitE[elim!]: "st\<turnstile>stmt.Exit\<longrightarrow>st"
+inductive_cases ProcessE[elim!]: "st\<turnstile>stmt.ProcessSt p\<longrightarrow>st1"
+inductive_cases SetStateE[elim!]: "st\<turnstile>stmt.SetStateSt st_name_option\<longrightarrow>st1"
+inductive_cases ResetE[elim!]: "st\<turnstile>stmt.ResetSt\<longrightarrow>st1"
+
+text "exec_func code_pred_intro lemmas"
+lemma [code_pred_intro]:
+"\<lbrakk>(f_name,res,vars,stmts) = (get_func_by_name st name);
+                  proxy_state = (gen_proxy_for_func st (f_name,res,vars,stmts));
+                  assign_param st assign_type.ColonEq params proxy_state as_proxy_state;
+                  as_proxy_state\<turnstile>stmts\<longrightarrow>st1;
+                  assign_param st1 assign_type.Conseq params st new_st;
+                  res = (get_cur_symbvar_by_name st1 f_name)\<rbrakk>\<Longrightarrow>
+                st\<turnstile>name,params\<longrightarrow>(new_st,res)"
+  by (auto intro: eval_exec_exec_func_assign_param.FuncStep)
+
+inductive_cases FuncE[elim!]:"st\<turnstile>name,params\<longrightarrow>(new_st,res)"
+
+text "param_assign code_pred_intro lemmas"
+lemma [code_pred_intro]:
+"assign_param base_st type [] st st"
+"\<lbrakk>base_st \<turnstile> exp \<rightarrow> (st,val);
+                       (if as_type = assign_type.ColonEq 
+                        then (assign_param base_st assign_type.ColonEq other (set_symbvar st name val) new_st)
+                        else (assign_param base_st assign_type.ColonEq other st new_st))\<rbrakk> \<Longrightarrow> 
+                      assign_param base_st assign_type.ColonEq ((param_assign.SymbolicVar name as_type exp)#other) st new_st"
+"\<lbrakk>base_st \<turnstile> exp \<rightarrow> (st,val);
+                       (if as_type = assign_type.Conseq 
+                        then (assign_param base_st assign_type.Conseq other st new_st) 
+                        else (assign_param base_st assign_type.Conseq other (set_symbvar st name val) new_st))  \<rbrakk> \<Longrightarrow> 
+                      assign_param base_st assign_type.Conseq ((param_assign.SymbolicVar name as_type exp)#other) st new_st"
+  by (auto intro: eval_exec_exec_func_assign_param.intros)
+
+inductive_cases AssignPE[elim!]: "assign_param base_st at pa st new_st"
 
 inductive 
   eval_state :: "[model_context,stacked_state,statement_result * model_context] \<Rightarrow> bool" ("_ \<turnstile> _ : _") where
-    StateStep : "\<lbrakk>(statement_result.Continue,st)\<turnstile>stm\<longrightarrow>(res,st1);
-                  (case res of 
-                    statement_result.Continue \<Rightarrow> 
-                      (case timeout_op of
+    StateStep : "\<lbrakk>st\<turnstile>stm\<longrightarrow>st1;
+                  (case timeout_op of
+                    None \<Rightarrow> (res,st2) = (res,st1)
+                    | (Some timeout) \<Rightarrow> 
+                      (case (extr_timeout_stmt st1 timeout) of 
                         None \<Rightarrow> (res,st2) = (res,st1)
-                      | (Some timeout) \<Rightarrow> 
-                          (case (extr_timeout_stmt st1 timeout) of 
-                            None \<Rightarrow> (res,st2) = (res,st1)
-                          | (Some stm1) \<Rightarrow> ((statement_result.Continue,st1)\<turnstile>stm1\<longrightarrow>(res,st2))))
-                  )\<rbrakk> \<Longrightarrow> 
+                        | (Some stm1) \<Rightarrow> (st1\<turnstile>stm1\<longrightarrow>st2)))\<rbrakk> \<Longrightarrow> 
                 st \<turnstile>(name,_,stm,timeout_op):(res,st2)"
 (*declare eval_state.intros [simp,intro]*)
 
@@ -258,11 +312,175 @@ inductive
                 (Suc n)\<Zspot>t:st\<turnstile>model\<mapsto>st2"
 
 
-code_pred eval.
+lemma comb_assoc:
+"st\<turnstile>stmt.Comb (stmt.Comb c1 c2) c3 \<longrightarrow> st1 \<longleftrightarrow> st\<turnstile>stmt.Comb c1 (stmt.Comb c2 c3) \<longrightarrow> st1"
+proof 
+  assume "st\<turnstile>stmt.Comb (stmt.Comb c1 c2) c3 \<longrightarrow> st1"
+  then obtain s1 s2 where
+    c1: "st\<turnstile>c1\<longrightarrow>s1" and
+    c2: "s1\<turnstile>c2\<longrightarrow>s2" and
+    c3: "s2\<turnstile>c3\<longrightarrow>st1" by auto
+  from c2 c3
+  have "s1\<turnstile>stmt.Comb c2 c3 \<longrightarrow>st1" by (rule Comb)
+  with c1
+  show "st\<turnstile>(stmt.Comb c1 (stmt.Comb c2 c3))\<longrightarrow>st1" by (rule Comb)
+next
+  assume "st\<turnstile>stmt.Comb c1 (stmt.Comb c2 c3)\<longrightarrow>st1"
+  then obtain s1 s2 where
+    c1: "st\<turnstile>c1\<longrightarrow>s1" and
+    c2: "s1\<turnstile>c2\<longrightarrow>s2" and
+    c3: "s2\<turnstile>c3\<longrightarrow>st1" by auto
+  from c1 c2
+  have "st\<turnstile>stmt.Comb c1 c2 \<longrightarrow>s2" by (rule Comb)
+  with c3
+  show "st\<turnstile>(stmt.Comb (stmt.Comb c1 c2) c3)\<longrightarrow>st1" by (simp add: Comb)
+qed
+
+lemma
+"st\<turnstile>stmt.IfSt b stmt.Blank stmt.Blank \<longrightarrow> st1 \<Longrightarrow> st =st1"
+  by blast
+  
+
+abbreviation equiv_c :: "stmt \<Rightarrow> stmt \<Rightarrow> bool" (infix "\<sim>" 50) where
+"c \<sim> c' \<equiv> (\<forall>s t. s\<turnstile>c\<longrightarrow>t = s\<turnstile>c'\<longrightarrow>t)"
+
+lemma sim_refl:  "c \<sim> c" by simp
+lemma sim_sym:   "(c \<sim> c') = (c' \<sim> c)" by auto
+lemma sim_trans: "c \<sim> c' \<Longrightarrow> c' \<sim> c'' \<Longrightarrow> c \<sim> c''" by auto
+
+lemma unfold_while:
+"(stmt.WhileSt b c) \<sim> (stmt.IfSt b (stmt.Comb c (stmt.WhileSt b c)) (stmt.Blank))" (is "?w \<sim> ?iw")
+proof -
+  have "st\<turnstile>?iw\<longrightarrow>st1" if assm: "st\<turnstile>?w\<longrightarrow>st1" for st st1
+  proof - 
+    from assm show ?thesis
+    proof cases
+      case LoopF
+      thus ?thesis by (simp add: Blank IfF)
+    next
+      case LoopT
+      thus ?thesis by (simp add: Comb IfT)
+    qed
+  qed
+  moreover
+  have "st\<turnstile>?w\<longrightarrow>st1" if assm: "st\<turnstile>?iw\<longrightarrow>st1" for st st1
+  proof -
+    from assm show ?thesis
+    proof cases
+      case IfF
+      thus ?thesis using LoopF by fastforce
+    next
+      case IfT
+      thus ?thesis using LoopT by force
+    qed
+  qed
+  ultimately
+  show ?thesis by meson
+qed
+
+lemma triv_if:
+"st\<turnstile>(stmt.IfSt b c c)\<longrightarrow>st1 \<Longrightarrow> st\<turnstile>c\<longrightarrow>st1"
+proof -
+  assume "st\<turnstile>(stmt.IfSt b c c)\<longrightarrow>st1"
+  then show ?thesis
+  proof cases
+    case IfF
+    thus ?thesis by blast
+  next
+    case IfT
+    thus ?thesis by blast
+  qed
+qed
+
+(*
+lemma triv_if:
+"(stmt.IfSt b c c) \<sim> c" (is "?w \<sim>?iw")
+proof -
+  have "st\<turnstile>?iw\<longrightarrow>st1" if assm: "st\<turnstile>?w\<longrightarrow>st1" for st st1
+  proof -
+    from assm show ?thesis
+    proof cases
+      case IfF
+      thus ?thesis by blast
+    next
+      case IfT
+      thus ?thesis by blast
+    qed
+  qed
+  moreover
+  have "st\<turnstile>?w\<longrightarrow>st1" if assm: "st\<turnstile>?iw\<longrightarrow>st1" for st st1
+  proof -
+    fix b::expr
+    from assm show ?thesis
+    proof (induction b arbitrary:?iw rule: eval_exec_exec_func_assign_param.induct)
+*)
+(*
+lemma comute_if:
+  "st\<turnstile>(stmt.IfSt b1 (stmt.IfSt b2 c11 c12) c2)\<longrightarrow>st1 \<longleftrightarrow> st\<turnstile>(stmt.IfSt b2 (stmt.IfSt b1 c11 c2) (stmt.IfSt b1 c12 c2))\<longrightarrow>st1" (is "?w\<longleftrightarrow>?iw")
+proof -
+  have ?iw if assm: ?w
+*)
+
+(*   
+lemma commute_if:
+  "(stmt.IfSt b1 (stmt.IfSt b2 c11 c12) c2) 
+    \<sim>
+   (stmt.IfSt b2 (stmt.IfSt b1 c11 c2) (stmt.IfSt b1 c12 c2))" (is "?w \<sim> ?iw")
+*)
+(*
+theorem
+  "st\<turnstile>c\<longrightarrow>st1 \<Longrightarrow> st\<turnstile>c\<longrightarrow>st2 \<Longrightarrow> st1=st2"
+proof (induction arbitrary: st2 rule: eval_exec_exec_func_assign_param.induct)
+*)
+
 declare eval_def [simp]
-code_pred (modes: i \<Rightarrow> i \<Rightarrow> o \<Rightarrow> bool) exec 
-  apply (smt (verit) exec.cases)
-  done
+(*
+code_pred (expected_modes: i \<Rightarrow> i \<Rightarrow> i \<Rightarrow> o)exec_func
+proof - 
+  case exec_func
+  from exec_func.prems show thesis
+  proof (cases)
+    case (FuncStep f_name vars stmts proxy_state as_proxy_state st1)
+    then show ?thesis by (simp add: exec_func.that(1))
+  qed
+qed
+
+code_pred (expected_modes: i \<Rightarrow> i \<Rightarrow> o)eval
+proof -
+  case eval
+  from eval.prems show thesis
+  proof (cases)
+    case (BinOp exp1 st1 val1 exp2 val2 bin_op)
+    from BinOp show thesis by (simp add: eval.that(1))
+  next
+    case (UnOp pexp val1 un_op)
+    from UnOp show thesis by (simp add: eval.that(2))
+  next
+    case (Const c)
+    from Const show thesis by (simp add: eval.that(3))
+  next
+    case (Var var_name)
+    from Var show thesis by (simp add: eval.that(4))
+  next
+    case (PSE p_name p_status)
+    from PSE show thesis by (simp add: eval.that(6))
+  next
+    case (FuncCall name as_list)
+    from FuncCall show thesis by (simp add: eval.that(7))
+  next
+    case (ArrayVar exp uu pos var_name)
+    from ArrayVar  show thesis by (auto simp add: eval.that(5))
+  qed
+  case exec_func
+  from exec_func.prems show thesis
+  proof (cases)
+    case (FuncStep f_name vars stmts proxy_state as_proxy_state st1)
+    then show ?thesis by (simp add: exec_func.that(1))
+  qed
+  
+qed
+  *)
+  
 
 (*
 proof -
